Langlib/Examples/MalbolgeUnshackled/loop.mu
@@ -1,0 +1,1 @@
+(CBA@?>=<;:9876543210/.-,+*)('&%$#"!~}|{zyxwvutsrqponmlkjihgfedcba`_^]\[ZYXWVUTSRQPONMLKJIHGFEDCBA@?>=<;:9876543210/.-,+*)('&%$#"!~}|{zyxwvutsrqponmlkjihKJ%dcba`_^]\[ZYXWVUTSRQPONMLKJIHGFEDCBA@Ç>=<;Å
